Work

ourlang.v
@@ -1,6 +1,11 @@
 
+Require Import CpdtTactics.
 From Coq Require Import Lists.List.
+From Coq Require Import Arith.PeanoNat.
+From Coq Require Import Arith.Peano_dec.
 Import ListNotations.
+
+Set Implicit Arguments.
 
 Definition append (A:Type) (l1 : list A) (l2 : list A) := concat [l1; l2].
 Notation "a ++ b" := (append a b).
@@ -12,29 +17,36 @@ Notation keyset := (list key).
 
 Inductive node : Type :=
 | N : key -> payload -> node.
+Hint Constructors node.
 
 Inductive operation : Type :=
-| inc : keyset -> operation.
+| inc : keyset -> operation
+| add : key -> payload -> operation.
+Hint Constructors operation.
 
 Definition target op :=
 match op with
 | inc ks => ks
+| add _ _ => []
 end.
 
 Definition final op : payload :=
 match op with
 | inc ks => 0
+| add k _ => k
 end.
 
 Inductive labeled_operation : Type :=
 | lo : label -> operation -> labeled_operation.
+Hint Constructors labeled_operation.
 
 Notation "l ->> o" := (lo l o) (at level 40).
 
-Notation result := payload.
+Notation result := nat.
 
 Inductive labeled_result : Type :=
 | lr : label -> result -> labeled_result.
+Hint Constructors labeled_result.
 
 Notation "l ->>> r" := (lr l r) (at level 40).
 
@@ -43,6 +55,7 @@ Notation rstream := (list labeled_result).
 
 Inductive station : Type :=
 | S : node -> ostream -> station.
+Hint Constructors station.
 
 Notation "<< n ; os >>" := (S n os).
 
@@ -50,6 +63,7 @@ Notation backend := (list station).
 
 Inductive config : Type :=
 | C : backend -> ostream -> rstream -> config.
+Hint Constructors config.
 
 Definition getKey (n : node) :=
 match n with
@@ -73,5 +87,92 @@ Inductive step : config -> config -> Prop :=
     c = C b os rs ->
     os = o :: os' ->
     b = (<<n1; os1>>)::b' ->
-    c --> C ((S n1 (os1 ++ [o]))::b') os' rs
+    c --> C (<<n1; (os1 ++ [o])>>::b') os' rs
+| S_Add : forall c b os rs os' l k v o,
+    c = C b os rs ->
+    os = o :: os' ->
+    o = l ->> add k v ->
+    c --> C (<<(N k v); []>> :: b) os' (l ->>> final (add k v) :: rs)
+| S_Inc : forall c b os rs b1 s1 s1' os1 os1' os1'' b2 k v ks l,
+    c = C b os rs ->
+    b = b1 ++ s1 :: b2 ->
+    s1 = <<(N k v); os1>> ->
+    os1 = l ->> inc ks :: os1'' ->
+    os1' = l ->> inc (remove Nat.eq_dec k ks) :: os1'' ->
+    s1' = <<(N k (v + 1)); os1'>> ->
+    In k ks ->
+    c --> C (b1 ++ s1' :: b2) os rs
+| S_Complete : forall c b os rs l n1 os1 os1' op b1 k,
+    c = C b os rs ->
+    b = b1 ++ [<<n1; os1>>] ->
+    os1 = l ->> op :: os1' ->
+    k = getKey n1 ->
+    not (In k (target op)) ->
+    c --> C (b1 ++ [<<n1; os1'>>]) os (l ->>> final op :: rs)
+(* S_Last *)
 where "c1 --> c2" := (step c1 c2).
+Hint Constructors step.
+Definition relation (X : Type) := X -> X -> Prop.
+Inductive multi {X : Type} (R : relation X) : relation X :=
+  | multi_refl : forall (x : X), multi R x x
+  | multi_step : forall (x y z : X),
+                    R x y ->
+                    multi R y z ->
+                    multi R x z.
+Hint Constructors multi.
+
+Notation multistep := (multi step).
+Notation "t1 '-->*' t2" := (multistep t1 t2) (at level 40).
+
+
+Example step_empty : (C [] [1 ->> inc []] []) --> (C [] [] [1 ->>> 0]).
+Proof using.
+  assert (0 = final (inc [])) by crush.
+  rewrite -> H.
+  apply S_Empty with (c := (C [] [1 ->> inc []] [])) (os := [1 ->> inc []]) (o := 1 ->> inc []); crush.
+Qed.
+
+Example step_first : (C [<<(N 1 1); []>>] [1 ->> inc []] []) --> (C [<<(N 1 1); [1 ->> inc []]>>] [] []).
+Proof using.
+  eapply S_First with (c := (C [<<(N 1 1); []>>] [1 ->> inc []] [])) (n1 := (N 1 1)) (o := 1 ->> inc []) (os1 := []); crush.
+Qed.
+
+Example step_add : (C [] [1 ->> add 1 0] []) --> (C [<<(N 1 0); []>>] [] [1 ->>> 1]).
+Proof using.
+  eapply S_Add; crush.
+Qed.
+
+Example step_addinc1 : (C [] [1 ->> add 1 0; 2 ->> inc [1]] []) --> (C [<<(N 1 0); []>>] [2 ->> inc [1]] [1 ->>> 1]).
+Proof using.
+  eapply S_Add; crush.
+Qed.
+
+Example step_addinc2 : (C [<<(N 1 0); []>>] [2 ->> inc [1]] [1 ->>> 1]) --> (C [<<(N 1 0); [2 ->> inc [1]]>>] [] [1 ->>> 1]).
+Proof using.
+  eapply S_First with (c := (C [<<(N 1 0); []>>] [2 ->> inc [1]] [1 ->>> 1])) (n1 := (N 1 0)) (o := 2 ->> inc [1]) (os1 := []); crush.
+Qed.
+
+Example step_addinc3 : (C [<<(N 1 0); [2 ->> inc [1]]>>] [] [1 ->>> 1]) --> (C [<<(N 1 1); [2 ->> inc []]>>] [] [1 ->>> 1]).
+Proof using.
+  eapply S_Inc with (c := (C [<<(N 1 0); [2 ->> inc [1]]>>] [] [1 ->>> 1])) (s1' := <<(N 1 1); [2 ->> inc []]>>) (b1 := []); crush.
+Qed.
+
+Example step_addinc4 : (C [<<(N 1 1); [2 ->> inc []]>>] [] [1 ->>> 1]) --> (C [<<(N 1 1); []>>] [] [2 ->>> 0; 1 ->>> 1]).
+Proof using.
+  assert (0 = final (inc [])) by crush.
+  rewrite -> H.
+  eapply S_Complete with (c := (C [<<(N 1 1); [2 ->> inc []]>>] [] [1 ->>> 1])) (n1 := (N 1 1)) (os1 := [2 ->> inc []]) (b1 := []); crush.
+Qed.
+
+Example step_addinc : (C [] [1 ->> add 1 0; 2 ->> inc [1]] []) -->* (C [<<(N 1 1); []>>] [] [2 ->>> 0; 1 ->>> 1]).
+Proof.
+  eapply multi_step.
+  apply step_addinc1.
+  eapply multi_step.
+  apply step_addinc2.
+  eapply multi_step.
+  apply step_addinc3.
+  eapply multi_step.
+  apply step_addinc4.
+  eapply multi_refl.
+Qed.
